proofs/transform/eliminate_algebraic_proofs/eliminate_algebraic_context.v
@@ -1,0 +1,476 @@
+(*Here we define the modified context from the [eliminate_algebraic] transformation*)
+Require Import Task eliminate_algebraic.
+
+Section Proofs.
+
+Variable (new_constr_name: funsym -> string).
+Variable keep_muts : mut_adt -> bool.
+
+Variable badnames : list string.
+(*TODO: assume that badnames includes all ids in gamma*)
+
+
+Variable (noind: typesym -> bool).
+
+Ltac replace_prop p1 p2 :=
+  let Hiff := fresh "Hiff" in 
+  assert (Hiff: p1 <-> p2); [| rewrite Hiff; clear Hiff].
+
+(*Step 1: Prove (syntactically) how gamma, delta, and goal are affected by transformation*)
+
+Section ContextSpecs.
+
+(*[add_param_decl]*)
+
+Lemma add_param_decl_delta tsk f: task_delta (add_param_decl tsk f) = task_delta tsk.
+Proof.
+  reflexivity.
+Qed.
+
+Lemma add_param_decl_gamma tsk f: task_gamma (add_param_decl tsk f) = abs_fun f :: task_gamma tsk.
+Proof.
+  reflexivity.
+Qed.
+
+Lemma add_param_decl_goal tsk f: task_goal (add_param_decl tsk f) = task_goal tsk.
+Proof.
+  reflexivity.
+Qed.
+
+(*[add_param_decls]*)
+
+Lemma add_param_decls_delta tsk l: task_delta (add_param_decls l tsk) = task_delta tsk.
+Proof.
+  revert tsk.
+  induction l; simpl; auto. intros tsk. rewrite IHl, add_param_decl_delta.
+  reflexivity.
+Qed.
+
+Lemma add_param_decls_gamma tsk l: task_gamma (add_param_decls l tsk) = rev (map abs_fun l) ++ task_gamma tsk.
+Proof.
+  revert tsk.
+  induction l; simpl; auto. intros tsk.
+  rewrite IHl, <- app_assoc, add_param_decl_gamma. reflexivity.
+Qed.
+
+Lemma add_param_decls_goal tsk l: task_goal (add_param_decls l tsk) = task_goal tsk.
+Proof.
+  revert tsk; induction l; simpl; auto; intros tsk. rewrite IHl, add_param_decl_goal. 
+  reflexivity.
+Qed.
+
+(*[add_axiom]*)
+
+Lemma add_axiom_gamma t n f: task_gamma (add_axiom t n f) = task_gamma t.
+Proof. reflexivity. Qed.
+
+Lemma add_axiom_delta t n f: task_delta (add_axiom t n f) = (n, f) :: task_delta t.
+Proof. reflexivity. Qed.
+
+(**[add_task_axioms]*)
+
+Lemma add_task_axioms_delta tsk ax:
+  task_delta (add_task_axioms tsk ax) = rev ax ++ task_delta tsk.
+Proof.
+  unfold add_task_axioms.
+  revert tsk. induction ax as [| h tl IH]; simpl; auto.
+  intros tsk. rewrite IH. simpl_task. destruct h; rewrite <- app_assoc; auto.
+Qed.
+
+Lemma add_task_axioms_gamma tsk ax:
+  task_gamma (add_task_axioms tsk ax) = task_gamma tsk.
+Proof.
+  unfold add_task_axioms.
+  revert tsk. induction ax as [| h tl IH]; simpl; auto.
+  intros tsk. rewrite IH. simpl_task. reflexivity.
+Qed.
+
+Lemma add_task_axioms_goal tsk ax:
+  task_goal (add_task_axioms tsk ax) = task_goal tsk.
+Proof.
+  unfold add_task_axioms.
+  revert tsk. induction ax as [| h tl IH]; simpl; auto.
+  intros tsk. rewrite IH. simpl_task. reflexivity.
+Qed.
+
+(*[add_ty_decl]*)
+
+Lemma add_ty_decl_gamma tsk ts: task_gamma (add_ty_decl tsk ts) = abs_type ts :: task_gamma tsk.
+Proof. reflexivity. Qed.
+
+Lemma add_ty_decl_delta tsk ts: task_delta (add_ty_decl tsk ts) = task_delta tsk.
+Proof. reflexivity. Qed.
+
+Lemma add_ty_decl_goal tsk ts: task_goal (add_ty_decl tsk ts) = task_goal tsk.
+Proof. reflexivity. Qed.
+
+(*[add_projections] (We do separately because of the nested induction - we convert
+  each [fold_left] to [fold_right])*)
+
+(*Should we just define it this way?*)
+(*Note, might need In version*)
+Lemma add_projections_delta {A B: Type} (tsk: task) (ts: A) (ty: B) (cs: list funsym):
+  task_delta (add_projections new_constr_name badnames tsk ts ty cs) =
+  (concat (map (fun c => (rev (map snd (projection_axioms new_constr_name badnames c ((projection_syms badnames c)))))) (rev cs))) ++
+  task_delta tsk.
+Proof.
+  Opaque projection_axioms. Opaque projection_syms. unfold add_projections. simpl.
+  rewrite <- fold_left_rev_right.
+  induction (rev cs) as [| c ctl IHc]; simpl; auto.
+  (*again, go to fold_right*) 
+  rewrite <- fold_left_rev_right.
+  rewrite <- map_rev.
+  induction (rev (projection_axioms new_constr_name badnames c (projection_syms badnames c))) as [| h t IH2]; simpl; auto.
+  rewrite add_axiom_delta. f_equal; auto. destruct (snd h); reflexivity.
+Qed.
+
+Lemma add_projections_gamma {A B: Type} (tsk: task) (ts: A) (ty: B) (cs: list funsym):
+  task_gamma (add_projections new_constr_name badnames tsk ts ty cs) =
+  map abs_fun (concat (map (fun c => rev (map fst (projection_axioms new_constr_name badnames c ((projection_syms badnames c))))) (rev cs))) ++
+  task_gamma tsk.
+Proof.
+  simpl. unfold add_projections. rewrite <- fold_left_rev_right.
+  induction (rev cs) as [|c ctl IH]; simpl; auto.
+  rewrite <- fold_left_rev_right.
+  rewrite map_app, <-  map_rev.
+  induction (rev (projection_axioms new_constr_name badnames c (projection_syms badnames c))) as [| h t IH2]; simpl; auto.
+  rewrite add_axiom_gamma, add_param_decl_gamma. f_equal.
+  rewrite IH2,  <- app_assoc. reflexivity.
+Qed. 
+
+Lemma add_projections_goal {A B: Type} (tsk: task) (ts: A) (ty: B) (cs: list funsym):
+  task_goal (add_projections new_constr_name badnames tsk ts ty cs) =
+  task_goal tsk.
+Proof.
+  simpl. unfold add_projections. rewrite <- fold_left_rev_right.
+  induction (rev cs) as [|c ctl IH]; simpl; auto.
+  rewrite <- fold_left_rev_right.
+  induction (rev (projection_axioms new_constr_name badnames c (projection_syms badnames c))) as [| h t IH2]; simpl; auto.
+Qed. 
+
+(*[add_axioms] - The first interesting part*)
+
+Opaque inversion_axiom.
+Opaque selector_axiom.
+Opaque discriminator_axioms.
+Opaque indexer_axiom.
+Opaque projection_axioms.
+Opaque projection_syms.
+Opaque add_projections.
+  
+(*NOTE: this is why the functional view of the axioms are helpful: we can easily
+  express the axioms*)
+
+Definition add_axioms_delta (ts: typesym) (cs: list funsym) :=
+[inversion_axiom new_constr_name badnames ts (adt_ty ts) cs] ++
+  (*Projections are trickiest*)
+  (concat (map (fun c => rev (map snd (projection_axioms new_constr_name badnames c ((projection_syms badnames c))))) (rev cs))) ++
+  rev (if single cs then nil else if negb (noind ts) then
+    snd (indexer_axiom new_constr_name badnames ts cs)
+    else if (length cs) <=? 16 then
+    discriminator_axioms new_constr_name badnames ts (adt_ty ts) cs
+    else nil) ++
+  (*selector*)
+  (if single cs then nil else rev (snd (selector_axiom new_constr_name badnames ts cs))).
+
+
+Lemma add_axioms_delta_eq (t: task) (ts: typesym) (cs: list funsym): 
+  task_delta (add_axioms new_constr_name badnames noind t (ts, cs)) =
+  add_axioms_delta ts cs ++ 
+  task_delta t.
+Proof.
+  unfold add_axioms_delta.
+  destruct t as [[gamma delta] goal].
+  unfold add_axioms.
+  unfold add_inversion.
+  simpl.
+  rewrite add_axiom_delta.
+  (*inversion axiom*)
+  f_equal.
+  rewrite <- !app_assoc.
+  (*projections*)
+  rewrite add_projections_delta. f_equal.
+  unfold add_indexer, add_selector, add_discriminator.
+  (*Now some case analysis*)
+  destruct (single cs); simpl; [rewrite add_param_decls_delta; reflexivity |].
+  destruct (noind ts); simpl; [destruct (length cs <=? 16)|]; simpl;
+  unfold add_selector_aux, add_indexer_aux;
+  repeat (rewrite !add_task_axioms_delta, !add_param_decl_delta; try rewrite !add_param_decls_delta);
+  reflexivity.
+Qed.
+
+Definition add_axioms_gamma (ts: typesym) (cs: list funsym) :=
+  (*projection symbols*)
+  map abs_fun (concat (map (fun c => rev (map fst (projection_axioms new_constr_name badnames c (projection_syms badnames c)))) (rev cs))) ++
+  (*indexer symbols*)
+  (if negb (single cs) && negb (noind ts) then [abs_fun (fst (indexer_axiom new_constr_name badnames ts cs))]
+    else nil) ++
+  (*selector symbols*)
+  (if negb (single cs) then [abs_fun (fst (selector_axiom new_constr_name badnames ts cs))] else nil) ++
+  (*constructor symbols*)
+  (rev (map abs_fun (map (new_constr new_constr_name badnames) cs))).
+
+
+Lemma add_axioms_gamma_eq (t: task) (ts: typesym) (cs: list funsym): 
+  task_gamma (add_axioms new_constr_name badnames noind t (ts, cs)) =
+  add_axioms_gamma ts cs ++ task_gamma t.
+Proof.
+  unfold add_axioms_gamma; rewrite <- !app_assoc.
+  destruct t as [[gamma delta] goal].
+  unfold add_axioms.
+  unfold add_inversion.
+  simpl.
+  rewrite add_axiom_gamma.
+  (*handle projections*)
+  rewrite add_projections_gamma.
+  f_equal.
+  unfold add_indexer, add_selector, add_discriminator.
+  (*case analysis*)
+  destruct (single cs); simpl; [rewrite add_param_decls_gamma; reflexivity|].
+  destruct (noind ts); simpl; unfold add_selector_aux, add_indexer_aux;
+  [destruct (length cs <=? 16); simpl|];
+  repeat (rewrite !add_task_axioms_gamma, !add_param_decl_gamma; try rewrite !add_param_decls_gamma);
+  reflexivity.
+Qed.
+
+(*The goal is the easiest*)
+Lemma add_axioms_goal (t: task) (ts: typesym) (cs: list funsym): 
+  task_goal (add_axioms new_constr_name badnames noind t (ts, cs)) = task_goal t.
+Proof.
+  destruct t as[[gamma delta] goal].
+  unfold add_axioms.
+  unfold add_inversion.
+  simpl.
+  rewrite add_projections_goal.
+  unfold add_indexer, add_selector, add_discriminator.
+  destruct (single cs); simpl; [rewrite add_param_decls_goal; reflexivity|].
+  destruct (noind ts); simpl;
+  unfold add_selector_aux, add_indexer_aux;
+  [destruct (length cs <=? 16)|]; simpl;
+  repeat (rewrite !add_task_axioms_goal, !add_param_decl_goal; try rewrite add_param_decls_goal); reflexivity.
+Qed.
+
+(*[comp_ctx]*)
+Opaque add_axioms.
+(*NOTE: the gamma is for rewriteT (TODO: see if we can eliminate gamma)
+  We will instantiate with full context.
+  In their implementation, they use the known_map from the current task
+  we fold over (OK because task is essentially a list, so we have all the previous
+  things in list) - not sure best way, for now separate context*)
+Definition comp_ctx_gamma (d: def) (gamma: context) : list def :=
+  match d with
+  | datatype_def m =>
+    concat (map (fun a => add_axioms_gamma (adt_name a) (adt_constr_list a)) (rev (typs m))) ++
+    (if keep_muts m then [datatype_def m] else (rev (map (fun a => abs_type (adt_name a)) (typs m))))
+  | _ => [(TaskGen.def_map (rewriteT' keep_muts new_constr_name badnames gamma) (rewriteF' keep_muts new_constr_name badnames gamma nil true) d)]
+  end.
+
+Lemma add_mut_gamma m tys tsk: task_gamma (add_mut m tys tsk) = 
+  datatype_def (mk_mut tys (m_params m) (m_nodup m))  :: task_gamma tsk.
+Proof. reflexivity. Qed.
+
+Lemma comp_ctx_gamma_eq (d: def) t (gamma: context) :
+  task_gamma (comp_ctx keep_muts new_constr_name badnames noind gamma d t) = 
+  comp_ctx_gamma d gamma ++ task_gamma t. 
+Proof.
+  unfold comp_ctx. destruct d; try reflexivity.
+  unfold comp_ctx_gamma.
+  (* destruct (keep_muts m)
+  destruct (partition _ (typs m)) as [dl_concr dl_abs]; simpl. *)
+  rewrite <- fold_left_rev_right. rewrite <- (map_rev _ (typs m)).
+  (*Need in multiple places*)
+  assert (Habs: forall dl, task_gamma
+    (fold_left
+    (fun (t1 : task) (a : alg_datatype) =>
+    add_ty_decl t1 (adt_name a)) dl t) = 
+    rev (map (fun a : alg_datatype => abs_type (adt_name a)) dl) ++
+    task_gamma t).
+  {
+    intros dl.
+    rewrite <- fold_left_rev_right, <- map_rev.
+    induction (rev dl) as [| h tl IH]; simpl; auto.
+    rewrite add_ty_decl_gamma. f_equal; auto.
+  }
+  induction (rev (typs m)) as [| hd tl IH]; simpl; auto.
+  - destruct (keep_muts m); simpl; auto.
+  - rewrite add_axioms_gamma_eq, <- !app_assoc.
+    f_equal.
+    rewrite IH, <- !app_assoc. reflexivity.
+Qed.
+
+(*Delta is easier: it adds nothing except axioms*)
+Definition comp_ctx_delta (d: def) : list (string * formula) :=
+  match d with
+  | datatype_def m =>
+    concat (map (fun a => add_axioms_delta (adt_name a) (adt_constr_list a)) (rev (typs m)))
+  | _ => nil
+  end.
+
+Lemma comp_ctx_delta_eq (d: def) t (gamma: context) :
+  task_delta (comp_ctx keep_muts new_constr_name badnames noind gamma d t) = 
+  comp_ctx_delta d ++ task_delta t.
+Proof.
+  Opaque add_axioms_delta.
+  unfold comp_ctx. destruct d; try reflexivity.
+  unfold comp_ctx_delta.
+  (* destruct (partition _ (typs m)) as [dl_concr dl_abs]; simpl. *)
+  rewrite <- fold_left_rev_right. rewrite <- (map_rev _ (typs m)).
+  assert (Habs: forall dl, task_delta (fold_left
+    (fun (t1 : task) (a : alg_datatype) =>
+    add_ty_decl t1 (adt_name a)) dl t) = 
+    task_delta t).
+  {
+    intros dl.
+    generalize dependent t.
+    induction dl as [| h t1 IH]; simpl; auto. intros tsk.
+    rewrite IH, add_ty_decl_delta.
+    reflexivity.
+  }
+  induction (rev (typs m)) as [| hd tl IH]; simpl; auto.
+  - destruct (keep_muts m); simpl; auto.
+  - rewrite add_axioms_delta_eq, <- !app_assoc. f_equal.
+    apply IH.
+Qed.
+
+Lemma comp_ctx_goal_eq (d: def) t (gamma: context) :
+  task_goal (comp_ctx keep_muts new_constr_name badnames noind gamma d t) = 
+  task_goal t.
+Proof.
+  unfold comp_ctx. destruct d; try reflexivity.
+  rewrite <- fold_left_rev_right. rewrite <- (map_rev _ (typs m)).
+  assert (Habs: forall dl, task_goal (fold_left
+    (fun (t1 : task) (a : alg_datatype) =>
+    add_ty_decl t1 (adt_name a)) dl t) = 
+    task_goal t).
+  {
+    intros dl.
+    generalize dependent t.
+    induction dl as [| h t IH]; simpl; auto. intros tsk.
+    rewrite IH, add_ty_decl_goal.
+    reflexivity.
+  }
+  induction (rev (typs m)) as [| hd tl IH]; simpl; auto.
+  - destruct (keep_muts m); simpl; auto.
+  - rewrite add_axioms_goal. apply IH.
+Qed.
+
+(*[fold_all_ctx]*)
+
+Definition fold_all_ctx_gamma t : context :=
+  concat (map (fun d => comp_ctx_gamma d (task_gamma t)) (rev (task_gamma t))).
+
+Lemma fold_all_ctx_gamma_eq t:
+  task_gamma (fold_all_ctx keep_muts new_constr_name badnames noind t) = fold_all_ctx_gamma t.
+Proof.
+  unfold fold_all_ctx, fold_all_ctx_gamma.
+  (*Basically, we need to split the task_gamma t up*)
+  remember (task_gamma t) as gamma.
+  (*Weird: if we rewrite without occurrence rewrites under binders but not with numbers*)
+  rewrite Heqgamma at 1 2.
+  clear Heqgamma.
+  rewrite <- fold_left_rev_right.
+  induction (rev (task_gamma t)); simpl; auto.
+  rewrite comp_ctx_gamma_eq.
+  f_equal; auto.
+Qed.
+
+Definition fold_all_ctx_delta t:= concat (map comp_ctx_delta (rev (task_gamma t))).
+
+Lemma fold_all_ctx_delta_eq t:
+  task_delta (fold_all_ctx keep_muts new_constr_name badnames noind t) = fold_all_ctx_delta t ++ task_delta t.
+Proof.
+  unfold fold_all_ctx, fold_all_ctx_delta.
+  remember (task_gamma t) as gamma.
+  rewrite Heqgamma at 1 2.
+  clear Heqgamma.
+  rewrite <- fold_left_rev_right.
+  induction (rev (task_gamma t)); simpl; auto.
+  rewrite comp_ctx_delta_eq.
+  rewrite <- app_assoc.
+  f_equal; auto.
+Qed.
+
+Lemma fold_all_ctx_goal_eq t:
+  task_goal (fold_all_ctx keep_muts new_constr_name badnames noind t) = task_goal t.
+Proof.
+  unfold fold_all_ctx.
+  remember (task_gamma t) as gamma.
+  rewrite Heqgamma at 1.
+  clear Heqgamma.
+  rewrite <- fold_left_rev_right.
+  induction (rev (task_gamma t)); simpl; auto.
+  rewrite comp_ctx_goal_eq.
+  assumption.
+Qed.
+
+End ContextSpecs.
+
+(*Some results about context*)
+
+(*TODO: generalize?*)
+Definition new_gamma (gamma: context) : context :=
+  concat (map (fun d => comp_ctx_gamma d gamma) (rev gamma)).
+(*NOTE: an easier definition for induction: we need to do induction only over gamma2, not gamma1*)
+Definition new_gamma_gen (g1 g2: context) : context :=
+  concat (map (fun d => comp_ctx_gamma d g1) g2).
+Lemma new_gamma_eq gamma: new_gamma gamma = new_gamma_gen gamma (rev gamma).
+Proof. reflexivity. Qed.
+
+
+(*TODO: move (from eliminate_inductive.v)*)
+Lemma mut_of_context_app l1 l2:
+  mut_of_context (l1 ++ l2) = mut_of_context l1 ++ mut_of_context l2.
+Proof.
+  induction l1; simpl; auto.
+  destruct a; simpl; auto. f_equal; auto.
+Qed.
+
+Lemma mut_of_context_abs_fun l:
+  mut_of_context (map abs_fun l) = nil.
+Proof.
+  induction l; simpl; auto.
+Qed.
+(*mutual ADTs of [new_gamma_gen] are subset of original*)
+Lemma mut_of_context_new_gamma (g1 g2: context) :
+  sublist (mut_of_context (new_gamma_gen g1 g2)) (mut_of_context g2).
+Proof.
+  induction g2 as [| d g2 IH]; simpl; [apply sublist_refl|].
+  unfold new_gamma_gen; simpl.
+  rewrite mut_of_context_app.
+  destruct d; simpl; auto.
+  (*Now prove that the [concat] part is empty, case in [keep_muts]*)
+  rewrite mut_of_context_app.
+  replace (mut_of_context (concat (map _ (rev (typs m))))) with (@nil mut_adt).
+  2: {
+    induction (rev (typs m)) as [| h t IH2]; simpl; auto.
+    rewrite mut_of_context_app, <- IH2, app_nil_r.
+    unfold add_axioms_gamma.
+    rewrite !mut_of_context_app.
+    rewrite <- map_rev.
+    rewrite !mut_of_context_abs_fun.
+    destruct (_ && _); destruct (negb (single _)); simpl; auto.
+  }
+  simpl.
+  destruct (keep_muts m).
+  - simpl. apply sublist_cons_l; auto.
+  - (*Here, abstract typesyms dont add to mut*)
+    replace (mut_of_context (rev (map _ _))) with (@nil mut_adt); simpl.
+    2: {
+      rewrite <- map_rev.
+      induction (rev (typs m)) as [| h t IH2]; simpl; auto. 
+    }
+    apply sublist_cons; auto.
+Qed.
+
+Lemma mut_in_ctx_new_gamma (g1 g2: context) (m: mut_adt):
+  mut_in_ctx m (new_gamma_gen g1 g2) ->
+  mut_in_ctx m g2.
+Proof.
+  unfold mut_in_ctx.
+  intros Hin.
+  apply in_bool_In in Hin.
+  apply In_in_bool.
+  apply mut_of_context_new_gamma in Hin. exact Hin.
+Qed.
+
+End Proofs.
