proofs/transform/eliminate_algebraic_proofs/eliminate_algebraic_proofs.v
@@ -1,0 +1,275 @@
+Require Import Task PatternProofs GenElts.
+Require Import compile_match eliminate_algebraic
+  eliminate_algebraic_context.
+Set Bullet Behavior "Strict Subproofs".
+
+(*TODO: should pre and post conditions be bools so we can check manually if need be?*)
+
+(*First condition we need: no recursive functions or inductive predicates*)
+(*TODO: prove for [eliminate_recursive]/[eliminate_definition]/[eliminate_inductive]*)
+Definition no_recfun_indpred_gamma (gamma: context) : bool :=
+  forallb (fun x =>
+    match x with
+    | recursive_def _ => false
+    | inductive_def _ => false
+    | _ => false
+    end) gamma.
+
+Definition no_recfun_indpred (t: task) : Prop :=
+  no_recfun_indpred_gamma (task_gamma t).
+
+(*Second condition: all patterns in non-recursive definitions, hyps, goals, are simple*)
+
+Definition funpred_def_simple_pats (f: funpred_def) : bool :=
+  match f with
+  | fun_def _ _ t => term_simple_pats t
+  | pred_def _ _ f => fmla_simple_pats f
+  end.
+
+Definition task_pat_simpl (t: task) : Prop :=
+  forallb (fun x =>
+    match x with
+    | nonrec_def fd => funpred_def_simple_pats fd
+    | _ => true
+    end) (task_gamma t) &&
+  forallb (fun x => fmla_simple_pats (snd x)) (task_delta t) &&
+  fmla_simple_pats (task_goal t).
+
+(*TODO: might be better for bools*)
+Definition task_and (P1 P2: task -> Prop) : task -> Prop :=
+  fun t => (P1 t /\ P2 t).
+
+(*Postcondition for *)
+
+(*TODO: what is ending condition? Do we need that ADTs are gone, or do we not care?
+  Maybe prove separately anyway*)
+(*For now, just conjoin 2 conditions*)
+Definition elim_alg_post: task -> Prop :=
+  task_and no_recfun_indpred task_pat_simpl.
+
+(*Theorems*)
+
+(*We want to prove both soundness and a postcondition for composition (TODO:
+  figure out what postcondition is but most likely either just no indpred and recfun
+  maybe no ADTs in list of [keep_tys] - for now, prove soundness)*)
+
+(*TODO: move*)
+
+Lemma sound_trans_pre_true (t: trans):
+  sound_trans t ->
+  sound_trans_pre (fun _ => True) t.
+Proof. 
+  unfold sound_trans, TaskGen.sound_trans, sound_trans_pre. intros Hsound tsk _ Hty Hallval.
+  apply Hsound; auto.
+Qed.
+
+Lemma sound_trans_weaken_pre (P1 P2: task -> Prop) (t: trans):
+  (forall t, P1 t -> P2 t) ->
+  sound_trans_pre P2 t ->
+  sound_trans_pre P1 t.
+Proof.
+  unfold sound_trans_pre.
+  intros Hp12 Hsound1 tsk Hp1 Hty Hallval.
+  apply Hsound1; auto.
+Qed. 
+
+Lemma trans_weaken_pre (P1 P2 Q1: task -> Prop) (t: trans):
+  (forall t, P1 t -> P2 t) ->
+  trans_pre_post P2 Q1 t ->
+  trans_pre_post P1 Q1 t.
+Proof.
+  unfold trans_pre_post.
+  intros; eauto.
+Qed.
+
+(*TODO: move to [compile_match]*)
+
+(*[trans_map] preserves no_recfun_indpred*)
+Lemma trans_map_pres_no_recfun_indpred f1 f2:
+  trans_pre_post no_recfun_indpred no_recfun_indpred (trans_map f1 f2).
+Proof.
+  unfold trans_pre_post, trans_map, TaskGen.trans_map, single_trans, TaskGen.task_map.
+  simpl.
+  unfold no_recfun_indpred.
+  intros t Hnorec Hty tr [Htr | []].
+  subst. simpl_task. unfold no_recfun_indpred_gamma in *.
+  rewrite forallb_map.
+  revert Hnorec. apply forallb_impl. intros x Hinx.
+  destruct x; auto.
+Qed.
+
+(*[compile_match] preserves [no_recfun_indpred]*)
+Lemma compile_match_pres_no_recfun_indpred:
+  trans_pre_post no_recfun_indpred no_recfun_indpred compile_match.
+Proof.
+  apply trans_map_pres_no_recfun_indpred.
+Qed.
+
+(*[compile_match] results in [task_pat_simpl] i.e. simplifies pattern matches (TODO: move)*)
+Lemma compile_match_simple:
+  trans_pre_post (fun _ => True) task_pat_simpl compile_match.
+Proof.
+  unfold trans_pre_post, compile_match, trans_map, TaskGen.trans_map, single_trans. simpl.
+  unfold TaskGen.task_map.
+  intros t _ Hty tr [Htr | []]; subst. unfold task_pat_simpl; simpl_task.
+  rewrite !forallb_map; simpl.
+  (*Need type info*)
+  destruct t as [[gamma delta] goal]; simpl in *.
+  inversion Hty. simpl_task.
+  bool_to_prop. split_all.
+  - apply forallb_forall. intros x Hinx.
+    destruct x; simpl; auto.
+    destruct f; simpl; auto.
+    + eapply rewriteT_simple_pats'; eauto.
+      apply nonrec_body_ty in Hinx; eauto.
+    + eapply rewriteF_simple_pats'; eauto.
+      apply nonrec_body_typed in Hinx; eauto.
+  - apply forallb_forall. intros x Hinx.
+    rewrite Forall_map, Forall_forall in task_delta_typed.
+    eapply rewriteF_simple_pats'; eauto.
+  - eapply rewriteF_simple_pats'; eauto.
+Qed. 
+
+(*Conjoin two postconditions*)
+Lemma task_post_combine (P1 Q1 Q2: task -> Prop) (t: trans) :
+  trans_pre_post P1 Q1 t ->
+  trans_pre_post P1 Q2 t ->
+  trans_pre_post P1 (task_and Q1 Q2) t.
+Proof.
+  unfold trans_pre_post, task_and. intros; split; eauto.
+Qed.
+
+(*Let's just prove typing first*)
+
+(*Idea: the transformation, broadly, goes like the following:
+  for each ADT (that should be axiomatized), generate all the new
+  function symbols, add them, add axioms, and add to state (to ensure axioms consistent)
+  then, rewrite terms/formulas using these symbols instead of pattern matching (rewriteT'/rewriteF')
+
+  The main result we need to prove is that if the new symbols are interpreted appropriately, 
+  then rewriteT'/rewriteF' is semantically equivalent (I think we do need both directions)
+  We will carefully interpret the new symbols:
+  basically, we have that (for delta), assuming 
+  (forall I', I', T(gamma) |= T(Delta) => I', T(gamma) |= T (g)), 
+  need to prove that (forall I, I, gamma |= Delta => I, gamma |= g)
+  so we take I, and make I' on result by interpreting each new function symbol in the "expected"
+  way (which we prove is consistent with the axioms). Then we prove if I, gamma |= Delta, 
+  then I', T(gamma) |= T(delta), so therefore, I', T(gamma) |= T(g), 
+  Then we need the reverse direction to show that I' |= T(g) iff I |= g (T is rewriteF' here).
+
+  NOTE: going to try at first to prove all at once and see what we need auxilliary, instead
+  of proving each intermediate transformation sound with a postcondition
+  *)
+
+Section Proofs.
+(*TODO: will we need to case on this?*)
+Variable (new_constr_name: funsym -> string).
+Variable keep_muts : mut_adt -> bool.
+
+Variable badnames : list string.
+(*TODO: assume that badnames includes all ids in gamma*)
+
+
+(* Variable (cc_maps: list funsym -> amap funsym funsym). *)
+Variable (noind: typesym -> bool).
+
+(*START: plan: formulate theorem correctly (with cc, cases) - should paramterize section
+  by them so we only have to prove once
+  Then prove similar for gamma (with new funsyms from e.g. selectors) - but need to
+  get order correct - e.g. have original gamma with a bunch of inorder declarations
+  goal is easy
+  Step 2: lift this to comp_ctx - delta is the same, gamma now replaces (some) types with
+  abstract types and adds same funsyms as above. Bit complicated is nonrec case if not eliminated
+  (b/c of alt-ergo really) - can't represnt as map I think because rewriteT should depend on gamma?
+  (NOTE: only depends on gamma bc we need to get constructors - could parameterize by map and add
+  to this lemma - constructor map is constant does not need fold - might be good to do this)
+  Step 3: go back to fold_comp - now know context, goals, etc, need to start proving
+  (e.g.) axioms true, well typed, etc*)
+
+Notation fold_all_ctx_gamma := (fold_all_ctx_gamma new_constr_name keep_muts badnames noind).
+Notation fold_all_ctx_delta := (fold_all_ctx_delta new_constr_name badnames noind).
+
+
+(*The core result: soundness of [fold_comp]
+  TODO: probably need to generalize from [empty_state]*)
+(*We need the precondition that pattern matches have been compiled away*)
+Theorem fold_comp_sound:
+  sound_trans_pre
+  (task_and no_recfun_indpred task_pat_simpl)
+  (fold_comp keep_muts new_constr_name badnames noind).
+Proof.
+  unfold sound_trans_pre.
+  intros tsk Hpre Hty Hallval.
+  unfold task_valid, TaskGen.task_valid in *.
+  split; auto.
+  intros gamma_valid Hty'.
+  (*Temp*) Opaque fold_all_ctx.
+  unfold fold_comp in Hallval.
+  (*Use gamma, delta, goal lemmas*)
+  rewrite fold_all_ctx_gamma_eq, fold_all_ctx_delta_eq, fold_all_ctx_goal_eq in Hallval.
+  set (newtsk := (fold_all_ctx_gamma tsk,
+    combine (map fst (fold_all_ctx_delta  tsk ++ task_delta tsk))
+      (map (rewriteF' keep_muts new_constr_name badnames (fold_all_ctx_gamma tsk) [] true)
+        (map snd (fold_all_ctx_delta  tsk ++ task_delta tsk))),
+    rewriteF' keep_muts new_constr_name badnames (fold_all_ctx_gamma tsk) [] true (task_goal tsk)))in *.
+  simpl in Hallval.
+  specialize (Hallval _ (ltac:(left; reflexivity))).
+  destruct Hallval as [Hty1 Hconseq1].
+  set (gamma1:= fold_all_ctx_gamma tsk) in *.
+  assert (Hgamma1: task_gamma newtsk = gamma1) by reflexivity.
+  assert (gamma1_valid: valid_context gamma1). {
+    inversion Hty1; auto.
+  }
+  specialize (Hconseq1 gamma1_valid Hty1).
+  assert (Hdelta: map snd (task_delta newtsk) = 
+    map (fun x => rewriteF' keep_muts new_constr_name badnames gamma1 [] true (snd x))
+      (fold_all_ctx_delta tsk ++ task_delta tsk)).
+  {
+    unfold newtsk. simpl_task. rewrite map_snd_combine; [rewrite map_map| solve_len].
+    reflexivity.
+  }
+  generalize dependent (task_delta_typed newtsk).
+  rewrite Hdelta; clear Hdelta (*TODO: need?*).
+  intros Hdelta1_typed Hconseq1.
+  assert (Hgoal: task_goal newtsk =
+    rewriteF' keep_muts new_constr_name badnames gamma1 [] true (task_goal tsk)) by reflexivity.
+  generalize dependent (task_goal_typed newtsk).
+  rewrite Hgoal; intros Hgoal1_typed Hconseq1.
+  (*So now we have to prove that if T(gamma), T(delta) |= T(goal), then gamma, delta |= goal
+    where T(gamma) = fold_all_ctx_gamma tsk, etc*)
+  unfold log_conseq_gen in *.
+  intros pd pdf pf pf_full Hdeltasat.
+  unfold satisfies in *.
+  intros vt vv.
+  (*Now we need to transform our pd and pf into the appropriate pd and pf on the modified
+    gamma*)
+
+  (*So we want to prove that the goal is satisfied.
+    so we need a lemma of the form: if formula_rep gamma1 (rewriteF' f), then
+      formula_rep gamma f (prob need iff) but for particular interp*)
+Admitted.
+
+Theorem eliminate_algebraic_sound : 
+  sound_trans_pre no_recfun_indpred
+  (eliminate_algebraic keep_muts new_constr_name badnames noind).
+Proof.
+  unfold eliminate_algebraic.
+  apply sound_trans_comp with (Q1:=
+    task_and no_recfun_indpred task_pat_simpl)
+  (P2:=task_and no_recfun_indpred task_pat_simpl).
+  - (*compile match soundness*)
+    apply sound_trans_weaken_pre with (P2:=fun _ => True); auto.
+    apply sound_trans_pre_true.
+    apply compile_match_valid.
+  - (*Sound trans of elim ADT (main part)*)
+    apply fold_comp_sound.
+  - (*pre and postconditions of [compile_match]*)
+    apply task_post_combine.
+    + apply compile_match_pres_no_recfun_indpred.
+    + apply trans_weaken_pre with (P2:=fun _ => True); auto.
+      apply compile_match_simple.
+  - apply compile_match_typed.
+  - auto.
+Qed.
+
+End Proofs.
